started on Instructions

src/Dafny/llvm.i.dfy
@@ -21,6 +21,41 @@ module LLVM_def {
         ok:bool)
 
 
+    // Taken from Vale -- modify for llvm
+    type shift_amount = s | 0 <= s < 32 // Some shifts allow s=32, but we'll be conservative for simplicity
+    datatype Shift =
+        | LSLShift(amount_lsl:shift_amount)
+        | LSRShift(amount_lsr:shift_amount)
+        | RORShift(amount_ror:shift_amount)
+
+    // datatype operand = OConst(n:uint32)
+        // | OReg(r:addr)
+        // | OShift(reg:addr, s:Shift)
+        // | OSymbol(sym:GlobalVar)
+        // | OSP
+        // | OLR
+    datatype operand = Value | LocalVar | GlobalVar
+
+    //---
+    //-----------------------------------------------------------------------------
+    // Instructions
+    //-----------------------------------------------------------------------------
+
+    datatype ins =
+    | ADD(t:Value, src1ADD:operand, src2ADD:operand)
+    | SUB(t:Value, src1ADD:operand, src2ADD:operand)
+    | BR(cond:bool, labelTrue:string,labelFalse:string)
+    | CALL() //needs work
+    | GETELEMENTPTR(t:Value,p:ptr,) //needs work
+    | ICMP()
+    | RET()
+    | SEXT()
+    | SHL()
+    | TRUN()
+    | ZEXT()
+    
+
+
     predicate State_Init(s:state)
     {
         s.ok 
@@ -40,5 +75,9 @@ module LLVM_def {
         ValidRegState(s.lvs,s.gvs) && ValidMemState(s.m)
     }
 
+    predicate ValidInstruction(s:state, ins:ins)
+    {
+        true
+    }
 
 }
